WIP ModelExtension.v

matching-logic/src/Theories/ModelExtension.v
@@ -234,8 +234,8 @@ Section with_syntax.
             (M : Model)
             (indec : forall (s : symbols),
               is_not_core_symbol s ->
-              forall (m : Domain M) ρₑ ρₛ,
-              Decision (m ∈ Minterp_inhabitant (patt_sym s) ρₑ ρₛ))
+              forall (m : Domain M) ρ,
+              Decision (m ∈ Minterp_inhabitant (patt_sym s) ρ))
             (R : Type)
             (fRM : R -> (Domain M) -> propset (Domain M + R)%type)
             (fMR : (Domain M) -> R -> propset (Domain M + R)%type)
@@ -325,11 +325,10 @@ Section with_syntax.
     := cel <$> (@fmap propset _ _ _ inl xs).
 
     (* Valuations lifted from the original model to the extended model. *)
-    Definition lift_val_e (ρₑ : @EVarVal _ M) : (@EVarVal _ Mext)
-    := λ (x : evar), (lift_value (ρₑ x)).
-
-    Definition lift_val_s (ρₛ : @SVarVal _ M) : (@SVarVal _ Mext)
-    := λ (X : svar), lift_set (ρₛ X).
+    Definition lift_val (ρ : @Valuation _ M) : (@Valuation _ Mext)
+    := mkValuation
+        (λ (x : evar), (lift_value (evar_valuation ρ x)))
+        (λ (X : svar), lift_set (svar_valuation ρ X)).
 
     Lemma lift_set_mono (xs ys : propset (Domain M)) :
         xs ⊆ ys <->
@@ -429,12 +428,12 @@ Section with_syntax.
     Lemma Mext_indec :
         forall (s : symbols),
             is_not_core_symbol s ->
-            forall (m : Domain Mext) ρₑ ρₛ,
-            Decision (m ∈ @Minterp_inhabitant Σ _ Mext (patt_sym s) (lift_val_e ρₑ) (lift_val_s ρₛ)).
+            forall (m : Domain Mext) ρ,
+            Decision (m ∈ @Minterp_inhabitant Σ _ Mext (patt_sym s) (lift_val ρ)).
     Proof.
         intros. unfold Minterp_inhabitant.
         rewrite eval_app_simpl.
-        unfold app_ext,lift_val_e,lift_val_s. simpl.
+        unfold app_ext,lift_val. simpl.
         destruct m.
         {
             right. intros HContra.
@@ -473,7 +472,7 @@ Section with_syntax.
             unfold new_app_interp in HContra3.
             repeat case_match; subst; auto; try set_solver.
         }
-        destruct (indec H d ρₑ ρₛ) as [Hin|Hnotin].
+        destruct (indec H d ρ) as [Hin|Hnotin].
         {
             left.
             unfold Minterp_inhabitant in Hin.
@@ -613,13 +612,12 @@ Section with_syntax.
 
 
         Lemma semantics_preservation_sym (s : symbols)
-            (ρₑ : @EVarVal _ M)
-            (ρₛ : @SVarVal _ M)
-            ρe0 ρs0
+            (ρ : @Valuation _ M)
+            ρ0
             :
             is_not_core_symbol s ->
-            @eval Σ Mext ρe0 ρs0 (patt_sym s) =
-            lift_set (@eval Σ M ρₑ ρₛ (patt_sym s)).
+            @eval Σ Mext ρ0 (patt_sym s) =
+            lift_set (@eval Σ M ρ (patt_sym s)).
         Proof.
             intros H.
             do 2 rewrite eval_sym_simpl.
@@ -633,13 +631,12 @@ Section with_syntax.
         Qed.
         
         Lemma semantics_preservation_inhabitant_set (s : symbols)
-            (ρₑ : @EVarVal _ M)
-            (ρₛ : @SVarVal _ M)
-            ρe0 ρs0
+            (ρ : @Valuation _ M)
+            ρ0
             :
             is_not_core_symbol s ->
-            @eval Σ Mext ρe0 ρs0 (patt_inhabitant_set (patt_sym s))
-            = lift_set (@eval Σ M ρₑ ρₛ (patt_inhabitant_set (patt_sym s))).
+            @eval Σ Mext ρ0 (patt_inhabitant_set (patt_sym s))
+            = lift_set (@eval Σ M ρ (patt_inhabitant_set (patt_sym s))).
         Proof.
             intros H.
             rename H into Hnc.
@@ -648,8 +645,8 @@ Section with_syntax.
             unfold_leibniz. 
             unfold patt_inhabitant_set.
             do 2 rewrite eval_app_simpl.
-            rewrite (semantics_preservation_sym ρₑ ρₛ);[assumption|].
-            remember (eval ρₑ ρₛ (patt_sym s)) as ps.
+            rewrite (semantics_preservation_sym ρ);[assumption|].
+            remember (eval ρ (patt_sym s)) as ps.
             unfold Sorts_Syntax.sym.
             do 2 rewrite eval_sym_simpl.
             unfold sym_interp at 1. simpl. unfold new_sym_interp.
@@ -693,14 +690,16 @@ Section with_syntax.
             }
         Qed.
 
-        Lemma update_evar_val_lift_val_e_comm
-            (ρₑ : @EVarVal _ M)
+        (*
+        Lemma update_evar_val_lift_val_comm
+            (ρ : @Valuation _ M)
             (x : evar)
             (d : Domain M)
             :
-            (@update_evar_val Σ Mext x (cel (inl d)) (lift_val_e ρₑ))
-            = lift_val_e (@update_evar_val Σ M x d ρₑ).
+            (@update_evar_val Σ Mext x (cel (inl d)) (lift_val ρ))
+            = lift_val (@update_evar_val Σ M x d ρ).
         Proof.
+            destruct ρ as [ρₑ ρₛ]. unfold update_evar_val. simpl.
             apply functional_extensionality.
             intros x'.
             unfold update_evar_val, lift_val_e,lift_value.
@@ -720,7 +719,7 @@ Section with_syntax.
             unfold update_svar_val,lift_val_s,lift_set.
             case_match; reflexivity.
         Qed.
-
+*)
         Lemma lift_set_fa_union (C : Type) (f : C -> propset (Domain M)) :
             lift_set (stdpp_ext.propset_fa_union f) = stdpp_ext.propset_fa_union (λ k, lift_set (f k)).
         Proof.
@@ -766,24 +765,24 @@ Section with_syntax.
             (sz : nat)
             :
             (
-                forall (ϕ : Pattern) (ρₑ : @EVarVal _ M) (ρₛ : @SVarVal _ M),
+                forall (ϕ : Pattern) (ρ : @Valuation _ M),
                 size' ϕ < sz ->
                 is_SData ϕ ->
                 well_formed ϕ ->
-                @eval Σ Mext (lift_val_e ρₑ) (lift_val_s ρₛ) ϕ
-                = lift_set (@eval Σ M ρₑ ρₛ ϕ)
+                @eval Σ Mext (lift_val ρ) ϕ
+                = lift_set (@eval Σ M ρ ϕ)
             )
             /\
             (
-                forall (ψ : Pattern) (ρₑ : @EVarVal _ M) (ρₛ : @SVarVal _ M),
+                forall (ψ : Pattern) (ρ : @Valuation _ M),
                 size' ψ < sz ->
                 is_SPredicate ψ ->
                 well_formed ψ ->
-                (@eval Σ Mext (lift_val_e ρₑ) (lift_val_s ρₛ) ψ = ∅
-                <-> @eval Σ M ρₑ ρₛ ψ = ∅)
+                (@eval Σ Mext (lift_val ρ) ψ = ∅
+                <-> @eval Σ M ρ ψ = ∅)
                 /\
-                (@eval Σ Mext (lift_val_e ρₑ) (lift_val_s ρₛ) ψ = ⊤
-                <-> @eval Σ M ρₑ ρₛ ψ = ⊤)
+                (@eval Σ Mext (lift_val ρ) ψ = ⊤
+                <-> @eval Σ M ρ ψ = ⊤)
             ).
         Proof.
             induction sz.
@@ -803,7 +802,7 @@ Section with_syntax.
                 split.
                 {
                     (* preservation of data patterns *)
-                    intros ϕ ρₑ ρₛ Hszϕ HSData Hwf.
+                    intros ϕ ρ Hszϕ HSData Hwf.
                     destruct HSData; simpl in Hszϕ.
                     {
                         (* patt_bott *)
@@ -857,7 +856,7 @@ Section with_syntax.
                         (* patt_sorted_neg (patt_sym s) ϕ *)
                         unfold patt_sorted_neg.
                         do 2 rewrite eval_and_simpl.
-                        rewrite (semantics_preservation_inhabitant_set ρₑ ρₛ);[assumption|].
+                        rewrite (semantics_preservation_inhabitant_set ρ);[assumption|].
                         do 2 rewrite eval_not_simpl.
                         rewrite IHszdata.
                         {
@@ -869,8 +868,8 @@ Section with_syntax.
                         {
                             wf_auto2.
                         }
-                        remember (eval ρₑ ρₛ (patt_inhabitant_set (patt_sym s))) as Xinh.
-                        remember (eval ρₑ ρₛ ϕ) as Xϕ.
+                        remember (eval ρ (patt_inhabitant_set (patt_sym s))) as Xinh.
+                        remember (eval ρ ϕ) as Xϕ.
                         clear HeqXinh HeqXϕ IHszpred IHszdata.
                         unfold_leibniz.
                         set_solver.
@@ -978,7 +977,7 @@ Section with_syntax.
 
                         rename H into Hspred.
                     
-                        destruct (classic (eval ρₑ ρₛ ψ = ∅)).
+                        destruct (classic (eval ρ ψ = ∅)).
                         {
                             rewrite IHszdata.
                             { lia. }
@@ -986,7 +985,7 @@ Section with_syntax.
                             { wf_auto2. }
                             clear HSData IHszdata. 
                             unfold_leibniz.
-                            specialize (IHszpred ψ ρₑ ρₛ ltac:(lia) ltac:(assumption) ltac:(wf_auto2)).
+                            specialize (IHszpred ψ ρ ltac:(lia) ltac:(assumption) ltac:(wf_auto2)).
                             destruct IHszpred as [Hsp1 Hsp2].
                             clear Hsp2.
                             destruct Hsp1 as [Hsp11 Hsp12].
@@ -1009,8 +1008,8 @@ Section with_syntax.
                                     wf_auto2.
                                 }
                             }
-                            specialize (IHszpred ψ ρₑ ρₛ ltac:(lia) ltac:(assumption) ltac:(wf_auto2)).
-                            specialize (IHszdata ϕ ρₑ ρₛ ltac:(lia) HSData ltac:(wf_auto2)).
+                            specialize (IHszpred ψ ρ ltac:(lia) ltac:(assumption) ltac:(wf_auto2)).
+                            specialize (IHszdata ϕ ρ ltac:(lia) HSData ltac:(wf_auto2)).
 
                             destruct IHszpred as [Hsp1 Hsp2].
                             clear Hsp1.
@@ -1059,7 +1058,7 @@ Section with_syntax.
                             apply elem_of_subseteq. intros x Hx.
                             rewrite elem_of_PropSet. rewrite elem_of_PropSet in Hx.
                             destruct Hx as [c Hc].
-                            destruct (Mext_indec H c ρₑ ρₛ) as [Hin|Hnotin].
+                            destruct (Mext_indec H c ρ) as [Hin|Hnotin].
                             {
                                 unfold Minterp_inhabitant in Hin.
                                 (* [c] comes from [Domain M] *)
@@ -1158,7 +1157,7 @@ Section with_syntax.
                                 2: { simpl. lia. }
 
                                 exists d.
-                                destruct (indec H d ρₑ ρₛ) as [Hin'|Hnotin'].
+                                destruct (indec H d ρ) as [Hin'|Hnotin'].
                                 2: {
                                     exfalso.
                                     unfold Minterp_inhabitant in Hnotin'.
@@ -1202,13 +1201,13 @@ Section with_syntax.
                             destruct Ha' as [a [Ha Ha']].
                             inversion Ha. clear Ha. subst.
                             rewrite elem_of_PropSet.
-                            destruct (indec H c ρₑ ρₛ).
+                            destruct (indec H c ρ).
                             2: {
                                 exfalso. clear -Ha'. set_solver.
                             }
                             exists (lift_value c).
                             rewrite update_evar_val_lift_val_e_comm.
-                            destruct (Mext_indec H (lift_value c) ρₑ ρₛ) as [Hin | Hnotin].
+                            destruct (Mext_indec H (lift_value c) ρ) as [Hin | Hnotin].
                             {
                                 rewrite IHszdata.
                                 4: { wf_auto2. }
@@ -1410,7 +1409,7 @@ Section with_syntax.
                     }
                 }
                 {   (* preservation of predicates *)
-                    intros ψ ρₑ ρₛ Hszϕ HSPred Hwf.
+                    intros ψ ρ Hszϕ HSPred Hwf.
                     destruct HSPred; simpl in Hszϕ.
                     {
                         (* patt_bott *)
@@ -1453,7 +1452,7 @@ Section with_syntax.
                         rewrite Htmp.
                         unfold new_app_interp.
                         unfold_leibniz.
-                        destruct (classic (eval ρₑ ρₛ ϕ = ∅)) as [Hempty|Hnonempty].
+                        destruct (classic (eval ρ ϕ = ∅)) as [Hempty|Hnonempty].
                         {
                             rewrite Hempty.
                             split.
@@ -1735,7 +1734,7 @@ Section with_syntax.
                                         intros x Hx.
                                         rewrite elem_of_PropSet.
                                         exists cdef.
-                                        assert (Hex : exists el, el ∈ eval ρₑ ρₛ ϕ).
+                                        assert (Hex : exists el, el ∈ eval ρ ϕ).
                                         {
                                             clear -Hnonempty.
                                             apply NNPP. intros HContra.
@@ -1800,13 +1799,13 @@ Section with_syntax.
                     {
                         (* patt_impl ψ₁ ψ₂*)
                         do 2 rewrite eval_imp_simpl.
-                        pose proof (IH1 := IHszpred ϕ₁ ρₑ ρₛ).
+                        pose proof (IH1 := IHszpred ϕ₁ ρ).
                         feed specialize IH1.
                         { lia. }
                         { assumption. }
                         { wf_auto2. }
                         destruct IH1 as [IH11 IH12].
-                        pose proof (IH2 := IHszpred ϕ₂ ρₑ ρₛ).
+                        pose proof (IH2 := IHszpred ϕ₂ ρ).
                         feed specialize IH2.
                         { lia. }
                         { assumption. }
@@ -1863,8 +1862,8 @@ Section with_syntax.
                                 destruct_and!.
                                 assumption.
                             }
-                            specialize (HSPred1 ρₑ ρₛ).
-                            specialize (HSPred2 ρₑ ρₛ).
+                            specialize (HSPred1 ρ).
+                            specialize (HSPred2 ρ).
                             split; intros H.
                             {
                                 destruct HSPred1 as [H1T|H1B],
@@ -1948,7 +1947,7 @@ Section with_syntax.
                         {
                             split; intros H'; intros c.
                             {
-                                destruct (indec H c ρₑ ρₛ) as [Hin|Hnotin].
+                                destruct (indec H c ρ) as [Hin|Hnotin].
                                 2: { reflexivity. }
                                 specialize (H' (lift_value c)).
                                 rewrite update_evar_val_lift_val_e_comm in H'.
@@ -1964,7 +1963,7 @@ Section with_syntax.
                                     wf_auto2.
                                 }
                                 destruct IHszpred as [IH1 IH2].
-                                destruct (Mext_indec H (lift_value c) ρₑ ρₛ) as [Hin'|Hnotin'].
+                                destruct (Mext_indec H (lift_value c) ρ) as [Hin'|Hnotin'].
                                 {
                                     apply IH1 in H'. apply H'.
                                 }
@@ -2017,7 +2016,7 @@ Section with_syntax.
                                 }
                             }
                             {
-                                destruct (Mext_indec H c ρₑ ρₛ) as [Hin|Hnotin].
+                                destruct (Mext_indec H c ρ) as [Hin|Hnotin].
                                 {
                                     unfold Minterp_inhabitant in Hin.
                                     rewrite eval_app_simpl in Hin.
@@ -2065,7 +2064,7 @@ Section with_syntax.
                                     destruct IHszpred as [IH1 IH2].
                                     rewrite IH1.
                                     specialize (H' d0).
-                                    destruct (indec H d0 ρₑ ρₛ) as [Hin'|Hnotin'].
+                                    destruct (indec H d0 ρ) as [Hin'|Hnotin'].
                                     {
                                         apply H'.
                                     }
@@ -2118,7 +2117,7 @@ Section with_syntax.
                             {
                                 specialize (H' stdpp.base.inhabitant).
                                 destruct H' as [c Hc].
-                                destruct (Mext_indec H c ρₑ ρₛ) as [Hin|Hnotin].
+                                destruct (Mext_indec H c ρ) as [Hin|Hnotin].
                                 {
                                     unfold Minterp_inhabitant in Hin.
                                     rewrite eval_app_simpl in Hin.
@@ -2152,7 +2151,7 @@ Section with_syntax.
                                     destruct Ha0 as [le' [re' [Hle' [Hre' Hle're']]]].
                                     rewrite elem_of_singleton in Hre'. subst re'.
                                     exists a0.
-                                    destruct (indec H a0 ρₑ ρₛ) as [Hin'|Hnotin'].
+                                    destruct (indec H a0 ρ) as [Hin'|Hnotin'].
                                     2: {
                                         exfalso. apply Hnotin'.
                                         unfold Minterp_inhabitant.
@@ -2200,10 +2199,10 @@ Section with_syntax.
                             {
                                 specialize (H' (@stdpp.base.inhabitant _ (Domain_inhabited M))).
                                 destruct H' as [c Hc].
-                                destruct (indec H c ρₑ ρₛ) as [Hin|Hnotin].
+                                destruct (indec H c ρ) as [Hin|Hnotin].
                                 {
                                     exists (lift_value c).
-                                    destruct (Mext_indec H (lift_value c) ρₑ ρₛ) as [Hin'|Hnotin'].
+                                    destruct (Mext_indec H (lift_value c) ρ) as [Hin'|Hnotin'].
                                     {
                                         rewrite update_evar_val_lift_val_e_comm.
                                         specialize (IHszpred (update_evar_val (fresh_evar ϕ) c ρₑ) ρₛ).
@@ -2318,7 +2317,7 @@ Section with_syntax.
                                 intros t.
                                 specialize (H' (stdpp.base.inhabitant)).
                                 destruct H' as [c Hc].
-                                destruct (Mext_indec H c ρₑ ρₛ) as [Hin|Hnotin].
+                                destruct (Mext_indec H c ρ) as [Hin|Hnotin].
                                 {
                                     unfold Minterp_inhabitant in Hin.
                                     rewrite eval_app_simpl in Hin.
@@ -2371,7 +2370,7 @@ Section with_syntax.
                                     apply SPred_is_pre_predicate in HSPred'.
                                     apply (@M_pre_predicate_evar_open Σ M ϕ (fresh_evar ϕ)) in HSPred'.
                                     exists a0.
-                                    destruct (indec H a0 ρₑ ρₛ) as [Hin'|Hnotin'].
+                                    destruct (indec H a0 ρ) as [Hin'|Hnotin'].
                                     {
                                         rewrite update_evar_val_lift_val_e_comm in Hc.
                                         intros HContra. apply Hc. clear Hc.
@@ -2418,7 +2417,7 @@ Section with_syntax.
                                 intros t.
                                 specialize (H' (@stdpp.base.inhabitant _ (Domain_inhabited M))).
                                 destruct H' as [c Hc].
-                                destruct (indec H c ρₑ ρₛ) as [Hin|Hnotin].
+                                destruct (indec H c ρ) as [Hin|Hnotin].
                                 {
                                     unfold Minterp_inhabitant in Hin.
                                     rewrite eval_app_simpl in Hin.
@@ -2446,7 +2445,7 @@ Section with_syntax.
                                     apply (@M_pre_predicate_evar_open Σ M ϕ (fresh_evar ϕ)) in HSPred'.
 
                                     exists (lift_value c).
-                                    destruct (Mext_indec H (lift_value c) ρₑ ρₛ) as [Hin'|Hnotin'].
+                                    destruct (Mext_indec H (lift_value c) ρ) as [Hin'|Hnotin'].
                                     {
                                         rewrite update_evar_val_lift_val_e_comm.
                                         unfold M_pre_predicate in HSPred'.
@@ -2527,7 +2526,7 @@ Section with_syntax.
                             intros H'.
                             {
                                 intros c.
-                                destruct (indec H c ρₑ ρₛ) as [Hin|Hnotin].
+                                destruct (indec H c ρ) as [Hin|Hnotin].
                                 {
                                     specialize (IHszpred (evar_open 0 (fresh_evar ϕ) ϕ) (update_evar_val (fresh_evar ϕ) c ρₑ) ρₛ).
                                     feed specialize IHszpred.
@@ -2544,7 +2543,7 @@ Section with_syntax.
                                     }
                                     destruct IHszpred as [IH1 IH2].
                                     specialize (H' (lift_value c)).
-                                    destruct (Mext_indec H (lift_value c) ρₑ ρₛ) as [Hin'|Hnotin'].
+                                    destruct (Mext_indec H (lift_value c) ρ) as [Hin'|Hnotin'].
                                     {
                                         rewrite update_evar_val_lift_val_e_comm in H'.
                                         apply IH2 in H'.
@@ -2600,7 +2599,7 @@ Section with_syntax.
                             }
                             {
                                 intros c.
-                                destruct (Mext_indec H c ρₑ ρₛ) as [Hin|Hnotin].
+                                destruct (Mext_indec H c ρ) as [Hin|Hnotin].
                                 2: { reflexivity. }
                                 unfold Minterp_inhabitant in Hin.
                                 rewrite eval_app_simpl in Hin.
@@ -2660,7 +2659,7 @@ Section with_syntax.
                                 }
                                 destruct IHszpred as [IH1 IH2].
                                 specialize (H' a1).
-                                destruct (indec H a1 ρₑ ρₛ) as [Hin'|Hnotin'].
+                                destruct (indec H a1 ρ) as [Hin'|Hnotin'].
                                 {
                                     apply IH2 in H'.
                                     apply H'.
